inverse ntt

lib/falcon/bv32_falcon_lemmas.i.dfy
@@ -56,7 +56,7 @@ module bv32_falcon_lemmas {
         a
     }
 
-    function lsize(view: forward_ntt.loop_view): (r: pow2_t)
+    function forward_lsize(view: forward_ntt.loop_view): (r: pow2_t)
         requires view.loop_view_wf();
         ensures r.full <= N.full
     {
@@ -114,8 +114,8 @@ module bv32_falcon_lemmas {
 
         requires N == pow2_t_cons(512, 9);
         requires forward_j_loop_inv(a, d, j, u, view);
-        requires t == lsize(view);
-        requires j < lsize(view).full;
+        requires t == view.lsize();
+        requires j < view.lsize().full;
         requires t.full < BASE_32;
         requires s5 == uint32_ls(uint32_add(t.full, j), 1);
         requires t6 == 2 * d.full;
@@ -322,10 +322,284 @@ module bv32_falcon_lemmas {
 
     lemma forward_j_loop_inv_post_lemma(a: seq<uint16>, d: pow2_t, j: nat, u: nat, view: forward_ntt.loop_view)
         requires forward_j_loop_inv(a, d, j, u, view);
-        requires j == lsize(view).full;
+        requires j == view.lsize().full;
         requires 0 <= view.hsize.exp <= N.exp;
         requires view.hsize == block_size(d);
         ensures forward_ntt.t_loop_inv(a, d, view.coefficients);
+    {
+        view.j_loop_inv_post_lemma(a, d, j);
+    }
+
+    function inverse_lsize(view: inverse_ntt.loop_view): (r: pow2_t)
+        requires view.loop_view_wf();
+        ensures r.full <= N.full
+    {
+        view.lsize()
+    }
+
+    predicate inverse_ntt_eval_all(a: seq<uint16>, coeffs: seq<uint16>)
+    {
+        && buff_is_nsized(a)
+        && buff_is_nsized(coeffs)
+        && inverse_ntt.ntt_eval_all(buff_as_nsized(a), buff_as_nsized(coeffs))
+    }
+
+    predicate inverse_t_loop_inv(a: seq<uint16>, d: pow2_t, coeffs: seq<uint16>)
+        requires 0 <= d.exp <= N.exp;
+    {
+        && buff_is_nsized(a)
+        && buff_is_nsized(coeffs)
+        && inverse_ntt.t_loop_inv(buff_as_nsized(a), d, buff_as_nsized(coeffs))
+    }
+
+    lemma inverse_t_loop_inv_pre_lemma(coeffs: seq<uint16>)
+        requires buff_is_nsized(coeffs);
+        ensures N.exp <= N.exp; // ??
+        ensures inverse_t_loop_inv(coeffs, N, coeffs);
+    {
+        inverse_ntt.t_loop_inv_pre_lemma(buff_as_nsized(coeffs));
+    }
+
+    lemma inverse_t_loop_inv_post_lemma(a: seq<uint16>, one: pow2_t, coeffs: seq<uint16>)
+        requires one.exp == 0 <= N.exp;
+        requires inverse_t_loop_inv(a, one, coeffs);
+        ensures inverse_ntt_eval_all(a, coeffs);
+    {
+        inverse_ntt.t_loop_inv_post_lemma(a, one, coeffs);
+    }
+
+    predicate inverse_s_loop_inv(a: seq<uint16>, d: pow2_t, j: nat, bi: nat, view: inverse_ntt.loop_view)
+    {
+        && buff_is_nsized(a)
+        && view.s_loop_inv(buff_as_nsized(a), d, j, bi)
+    }
+
+    lemma inverse_s_loop_inv_pre_lemma(
+        a: seq<uint16>,
+        d: pow2_t,
+        j: nat,
+        t: pow2_t,
+        u: nat,
+        ot3: uint32,
+        t3: uint32,
+        t6: uint32,
+        s5: uint32,
+        view: inverse_ntt.loop_view)
+
+        requires N == pow2_t_cons(512, 9);
+        requires inverse_j_loop_inv(a, d, j, u, view);
+        requires t == view.lsize();
+        requires j < view.lsize().full;
+        requires t.full < BASE_32;
+        requires s5 == uint32_ls(uint32_add(t.full, j), 1);
+        requires t6 == 2 * d.full;
+        requires ot3 == 2 * u;
+        requires t3 == uint32_add(ot3, t6);
+
+        ensures inverse_s_loop_inv(a, d, j, 0, view);
+        ensures s5 == (t.full + j) * 2; 
+        ensures t.full + j < N.full;
+        ensures t3 == 2 * u + 2 * d.full;
+        ensures rev_omega_inv_powers_mont_table()[t.full + j] == 
+            mqmul(rev_omega_inv_powers_x_value(2 * j, d), R);
+    {
+        view.s_loop_inv_pre_lemma(buff_as_nsized(a), d, j);
+        rev_omega_inv_powers_mont_table_lemma(t, d, j);
+        assert uint32_add(t.full, j) == t.full + j;
+        ls1_is_double(t.full + j);
+        // rev_omega_inv_powers_mont_table_lemma(t, d, j);
+
+        assert u == j * (2 * d.full);
+        assert d == view.hcount();
+
+        calc {
+            j * (2 * d.full) + d.full;
+            <= 
+            {
+                LemmaMulInequality(j, 512, 2 * d.full);
+            }
+            512 * (2 * d.full) + d.full;
+        }
+    }
+
+    lemma inverse_s_loop_inv_post_lemma(
+        a: seq<uint16>,
+        d: pow2_t,
+        j: nat,
+        u: uint32,
+        bi: nat,
+        ot3: uint32,
+        t3: uint32,
+        t6: uint32,
+        view: inverse_ntt.loop_view)
+    
+        requires N == pow2_t_cons(512, 9);
+        requires bi == d.full;
+        requires t6 == 2 * d.full;
+        requires u == j * (2 * d.full);
+        requires inverse_s_loop_inv(a, d, j, bi, view);
+        requires ot3 == 2 * u + 2 * d.full;
+        requires t3 == uint32_add(ot3, t6);
+        ensures t3 == 2 * (u + 2 * d.full);
+        ensures inverse_j_loop_inv(a, d, j + 1, u + 2 * d.full, view);
+    {
+        view.s_loop_inv_post_lemma(buff_as_nsized(a), d, j, bi);
+
+        assert u + 2 * d.full == (j + 1) * (2 * d.full) by {
+            LemmaMulProperties();
+        }
+
+        calc == {
+            ot3 + t6;
+            2 * u + 2 * d.full + 2 * d.full;
+            2 * (j * (2 * d.full)) + 2 * d.full + 2 * d.full;
+            {
+                LemmaMulProperties();
+            }
+            (2 * j + 2) * (2 * d.full);
+        }
+
+        assert d == view.hcount();
+
+        calc {
+            (2 * j + 2) * (2 * d.full);
+            <= 
+            {
+                LemmaMulInequality(2 * j + 2, 1024, 2 * d.full);
+            }
+            1024 * (2 * d.full);
+            <
+            {
+                assert d.full <= 512;
+            }
+            BASE_31;
+        }
+    }
+
+    lemma inverse_s_loop_index_lemma(
+        a: seq<uint16>,
+        d: pow2_t,
+        j: nat,
+        bi: nat,
+        s4: uint32,
+        s2: uint32,
+        t4: uint32,
+        t5: uint32,
+        t6: uint32,
+        view: inverse_ntt.loop_view)
+        returns (s: nat)
+
+        requires inverse_s_loop_inv(a, d, j, bi, view);
+        requires bi < d.full
+        requires s2 == 2 * bi + 2 * (j * (2 * d.full)); 
+        requires flat.ptr_admissible_32(heap_b32_index_ptr(s4, N.full / 2 - 1));
+        requires t4 == uint32_add(s4, s2);
+        requires t5 == uint32_add(t4, t6);
+        requires t6 == 2 * d.full;
+
+        ensures s == bi + (2*j) * d.full;
+        ensures t4 == s4 + 2 * s;
+        ensures t5 == s4 + 2 * (s + d.full);
+        ensures s + d.full < N.full;
+        ensures a[s] == level_points_view(a, view.hsize)[bi][2*j];
+        ensures s == point_view_index(bi, 2*j, view.hsize);
+        ensures a[s+d.full] == level_points_view(a, view.hsize)[bi][2*j+1];
+        ensures s+d.full == point_view_index(bi, 2*j+1, view.hsize);
+    {
+        s := view.higher_points_view_index_lemma(buff_as_nsized(a), d, j, bi);
+        assert 2 * (bi + (2*j) * d.full) == 2 * bi + 2 * (j * (2 * d.full)) by {
+            LemmaMulProperties();
+        }
+    }
+
+    predicate inverse_s_loop_update(
+        a: seq<uint16>,
+        a': seq<uint16>,
+        d: pow2_t,
+        j: nat,
+        bi: nat,
+        s: nat,
+        e: uint32,
+        o: uint32,
+        view: inverse_ntt.loop_view)
+
+        requires inverse_s_loop_inv(a, d, j, bi, view);
+        requires bi < d.full
+    {
+        && e < Q
+        && o < Q
+        && |a'| == |a|
+        && s + d.full < |a|
+        && a'[s + d.full] == o
+        && a'[s] == e
+        && a' == a[s + d.full := o][s := e]
+        && assert buff_is_nsized(a') by {
+            reveal buff_is_nsized();
+        }
+        && view.s_loop_update(buff_as_nsized(a), buff_as_nsized(a'), d, j, bi)
+    }
+
+    lemma inverse_s_loop_inv_peri_lemma(a: seq<uint16>,
+        a': seq<uint16>,
+        d: pow2_t,
+        j: nat,
+        bi: nat,
+        s: nat,
+        e: uint32,
+        o: uint32,
+        view: inverse_ntt.loop_view)
+
+        requires inverse_s_loop_inv(a, d, j, bi, view);
+        requires bi < d.full
+        requires inverse_s_loop_update(a, a', d, j, bi, s, e, o, view);
+        ensures inverse_s_loop_inv(a', d, j, bi+1, view);
+    {
+        view.s_loop_inv_peri_lemma(a, a', d, j, bi);
+        assert buff_is_nsized(a') by {
+            reveal buff_is_nsized();
+        }
+    }
+
+    lemma inverse_higher_points_view_index_lemma(a: seq<uint16>, d: pow2_t, j: nat, bi: nat, view: inverse_ntt.loop_view)
+        returns (s: nat)
+    
+        requires inverse_s_loop_inv(a, d, j, bi, view);
+        requires bi < d.full
+        ensures s == bi + (2*j) * d.full;
+        ensures s + d.full < N.full;
+        ensures a[s] ==
+            level_points_view(buff_as_nsized(a), view.hsize)[bi][2*j];
+        ensures s == point_view_index(bi, 2*j, view.hsize);
+        ensures a[s+d.full] ==
+            level_points_view(buff_as_nsized(a), view.hsize)[bi][2*j+1];
+        ensures s+d.full == point_view_index(bi, 2*j+1, view.hsize);
+    {
+        s := view.higher_points_view_index_lemma(buff_as_nsized(a), d, j, bi);
+    }
+
+    predicate inverse_j_loop_inv(a: seq<uint16>, d: pow2_t, j: nat, u: nat, view: inverse_ntt.loop_view)
+    {
+        && buff_is_nsized(a)
+        && u == j * (2 * d.full)
+        && view.j_loop_inv(buff_as_nsized(a), d, j)
+    }
+
+    lemma inverse_j_loop_inv_pre_lemma(a: seq<uint16>, d: pow2_t, view: inverse_ntt.loop_view)
+        requires 0 <= d.exp < N.exp;
+        requires inverse_t_loop_inv(a, pow2_double(d), view.coefficients);
+        requires view.loop_view_wf();
+        requires view.hsize == block_size(d);
+        ensures inverse_j_loop_inv(a, d, 0, 0, view);
+    {
+        view.j_loop_inv_pre_lemma(buff_as_nsized(a), d);
+    }
+
+    lemma inverse_j_loop_inv_post_lemma(a: seq<uint16>, d: pow2_t, j: nat, u: nat, view: inverse_ntt.loop_view)
+        requires inverse_j_loop_inv(a, d, j, u, view);
+        requires j == view.lsize().full;
+        requires 0 <= view.hsize.exp <= N.exp;
+        requires view.hsize == block_size(d);
+        ensures inverse_ntt.t_loop_inv(a, d, view.coefficients);
     {
         view.j_loop_inv_post_lemma(a, d, j);
     }
